update to BoolSpec based Decidable.v, annotate all assumption records with Prop, move varname_eq_dec from assumptions to parameters

compiler/src/FlatToRiscvLiterals.v
@@ -12,7 +12,7 @@ Require Import compiler.GoFlatToRiscv.
 Require Import compiler.EmitsValid.
 Require Import compiler.FlatToRiscvDef.
 Require Import compiler.FlatToRiscvCommon.
-
+Require Import coqutil.Tactics.autoforward.
 
 Section FlatToRiscvLiterals.
   Context {p: FlatToRiscv.parameters}.
@@ -27,53 +27,13 @@ Section FlatToRiscvLiterals.
 
   Definition updateMetricsForLiteral v initialMetrics : MetricLog :=
     let cost :=
-        if dec (- 2 ^ 11 <= v < 2 ^ 11)
+        if ((- 2 ^ 11 <=? v)%Z && (v <? 2 ^ 11)%Z)%bool
         then 1
         else
-          if dec (width = 32 \/ - 2 ^ 31 <= v < 2 ^ 31)
+          if ((width =? 32)%Z || (- 2 ^ 31 <=? v)%Z && (v <? 2 ^ 31)%Z)%bool
           then 2
           else 8 in
     addMetricInstructions cost (addMetricLoads cost initialMetrics).
-
-  Ltac update_metrics_invert :=
-    intros;
-    unfold updateMetricsForLiteral in *;
-    repeat match goal with
-           | H: ?P |- context[dec(?P)] =>
-             let H' := fresh "H'" in
-             destruct (dec P) as [|H']; [|exfalso; apply H'; apply H]
-           | H: ~?P |- context[dec(?P)] =>
-             let H'  := fresh "H'" in
-             destruct (dec P) as [H'|]; [exfalso; apply H; apply H'|]
-           end;
-    reflexivity.
-
-  Lemma invert_update_metrics_for_literal_1: forall v initialMetrics,
-    -2 ^ 11 <= v < 2 ^ 11 ->
-    updateMetricsForLiteral v initialMetrics =
-    addMetricInstructions 1 (addMetricLoads 1 initialMetrics).
-  Proof. update_metrics_invert. Qed.
-
-  Lemma invert_update_metrics_for_literal_2: forall v initialMetrics,
-    ~(-2 ^ 11 <= v < 2 ^ 11) ->
-    width = 32 \/ -2 ^ 31 <= v < 2 ^ 31 ->
-    updateMetricsForLiteral v initialMetrics =
-    addMetricInstructions 2 (addMetricLoads 2 initialMetrics).
-  Proof. update_metrics_invert. Qed.
-
-  Lemma invert_update_metrics_for_literal_8: forall v initialMetrics,
-    ~(-2 ^ 11 <= v < 2 ^ 11) ->
-    ~(width = 32 \/ -2 ^ 31 <= v < 2 ^ 31)->
-    updateMetricsForLiteral v initialMetrics =
-    addMetricInstructions 8 (addMetricLoads 8 initialMetrics).
-  Proof. update_metrics_invert. Qed.
-
-  Ltac bound_for_literal P :=
-    match goal with
-    | H : updateMetricsForLiteral _ _ = ?finalMetrics |- _ =>
-      rewrite P in H; [|assumption..];
-      subst finalMetrics; repeat split; solve_MetricLog
-    end.
 
   Lemma update_metrics_for_literal_bounded: forall v initialMetrics finalMetrics,
       updateMetricsForLiteral v initialMetrics = finalMetrics ->
@@ -82,12 +42,11 @@ Section FlatToRiscvLiterals.
       finalMetrics.(stores) <= initialMetrics.(stores) /\
       finalMetrics.(jumps) <= initialMetrics.(jumps).
   Proof.
-    intros.
-    destruct (dec (- 2 ^ 11 <= v < 2 ^ 11));
-      [|destruct (dec (width = 32 \/ - 2 ^ 31 <= v < 2 ^ 31))].
-    - bound_for_literal invert_update_metrics_for_literal_1.
-    - bound_for_literal invert_update_metrics_for_literal_2.
-    - bound_for_literal invert_update_metrics_for_literal_8.
+    intros. subst.
+    unfold updateMetricsForLiteral.
+    destruct initialMetrics.
+    simpl.
+    repeat (destruct_one_match; try blia).
   Qed.
 
   Ltac match_apply_runsTo :=
@@ -102,6 +61,22 @@ Section FlatToRiscvLiterals.
            | _: ?x = _ |- _ => subst x
            | _: _ = ?x |- _ => subst x
            end.
+
+  Ltac post_destr db :=
+    repeat match goal with
+           | E: (_ && _)%bool = true |- _ =>
+             let E1 := fresh E in let E2 := fresh E in
+             apply andb_prop in E; destruct E as [E1 E2];
+             autoforward_in db E1;
+             autoforward_in db E2
+           end.
+
+  (* mark as Instance? *)
+  Lemma andb_spec: forall b1 b2,
+      BoolSpec (b1 = true /\ b2 = true) (b1 = false \/ b2 = false) (b1 && b2)%bool.
+  Proof.
+    intros. destruct b1; destruct b2; constructor; auto.
+  Qed.
 
   Lemma compile_lit_correct_full: forall (initialL: RiscvMachineL) post x v R,
       initialL.(getNextPc) = add initialL.(getPc) (word.of_Z 4) ->
@@ -124,17 +99,21 @@ Section FlatToRiscvLiterals.
     simpl in *.
     destruct_RiscvMachine initialL.
     subst.
-    unfold compile_lit in *.
-    destruct (dec (- 2 ^ 11 <= v < 2 ^ 11));
-      [|destruct (dec (width = 32 \/ - 2 ^ 31 <= v < 2 ^ 31))].
+    unfold compile_lit, updateMetricsForLiteral in *.
+    destruct_one_match_hyp; [|destruct_one_match_hyp]; post_destr typeclass_instances.
     - unfold compile_lit_12bit in *.
-      rewrite invert_update_metrics_for_literal_1 in N; [|assumption].
       run1det.
       simpl_word_exprs word_ok.
       match_apply_runsTo.
-      erewrite signExtend_nop; eauto; blia.
-    - unfold compile_lit_32bit in *.
-      rewrite invert_update_metrics_for_literal_2 in N; [|assumption..].
+      erewrite signExtend_nop; eauto; try blia.
+    - (* TODO this step should be automatic *)
+      assert (width = 32 \/ - 2 ^ 31 <= v < 2 ^ 31). {
+        clear -E0 h.
+        apply Bool.orb_true_iff in E0. destruct E0 as [E0 | E0].
+        - autoforward_in typeclass_instances E0. auto.
+        - post_destr typeclass_instances. auto.
+      }
+      unfold compile_lit_32bit in *.
       simpl in P.
       run1det. run1det.
       match_apply_runsTo.
@@ -150,8 +129,8 @@ Section FlatToRiscvLiterals.
           clear. destruct width_cases; rewrite H; reflexivity.
         }
         rewrite! signExtend_alt_bitwise by (reflexivity || assumption).
-        clear -Wpos o.
-        destruct o as [E | B ].
+        clear -Wpos H.
+        destruct H as [E | B ].
         * rewrite E. unfold signExtend_bitwise. Zbitwise.
         * unfold signExtend_bitwise. Zbitwise.
           (* TODO these should also be solved by Zbitwise *)
@@ -175,7 +154,6 @@ Section FlatToRiscvLiterals.
       + solve_word_eq word_ok.
       + solve_word_eq word_ok.
     - unfold compile_lit_64bit, compile_lit_32bit in *.
-      rewrite invert_update_metrics_for_literal_8 in N; [|assumption..].
       match type of EV with
       | context [ Xori _ _ ?a ] => remember a as mid
       end.
@@ -201,9 +179,9 @@ Section FlatToRiscvLiterals.
       + rewrite! map.put_put_same. f_equal. subst.
         apply word.unsigned_inj.
         assert (width = 64) as W64. {
-          clear -n0.
+          clear -E0.
           destruct width_cases as [E | E]; rewrite E in *; try reflexivity.
-          exfalso. apply n0. left. reflexivity.
+          exfalso. simpl in E0. discriminate E0.
         }
         (repeat rewrite ?word.unsigned_of_Z, ?word.unsigned_xor, ?word.unsigned_slu);
         unfold word.wrap;
