compiler/src/util/ListLib.v
@@ -6,16 +6,18 @@ Require Import coqutil.Z.Lia.
 
 Section ListSet.
   Context {E: Type}.
-  Context {eeq: DecidableEq E}.
+  Context (eeq: E -> E -> bool).
+
+  Definition removeb(e: E)(l: list E): list E := filter (fun e' => negb (eeq e e')) l.
 
   Definition list_union(A B: list E): list E :=
-    fold_left (fun res a => if in_dec eeq a res then res else a :: res) A B.
+    fold_left (fun res a => if find (eeq a) res then res else a :: res) A B.
 
   Definition list_intersect(A B: list E): list E :=
-    fold_left (fun res a => if in_dec eeq a B then a :: res else res) A nil.
+    fold_left (fun res a => if find (eeq a) B then a :: res else res) A nil.
 
   Definition list_diff(A B: list E): list E :=
-    fold_left (fun res b => remove eeq b res) B A.
+    fold_left (fun res b => removeb b res) B A.
 
   Lemma length_list_union: forall (l1 l2: list E),
       (length (list_union l1 l2) <= length l1 + length l2)%nat.
@@ -27,17 +29,18 @@ Section ListSet.
   Qed.
 End ListSet.
 
-Lemma remove_In_ne{A: Type}{eqd: DecidableEq A}: forall (l: list A) (f1 f2: A),
+Lemma remove_In_ne{A: Type}(aeqb: A -> A -> bool){aeqb_spec: EqDecider aeqb}:
+  forall (l: list A) (f1 f2: A),
       In f1 l ->
       f1 <> f2 ->
-      In f1 (remove eqd f2 l).
+      In f1 (removeb aeqb f2 l).
 Proof.
   induction l; intros.
   - inversion H.
   - simpl in *. destruct H.
     + subst a.
-      destruct (eqd f2 f1); try congruence. simpl. auto.
-    + destruct (eqd f2 a).
+      destr (aeqb f2 f1); try congruence. simpl. auto.
+    + destr (aeqb f2 a); simpl.
       * subst a. eauto.
       * simpl. eauto.
 Qed.
@@ -77,7 +80,7 @@ Proof.
 Qed.
 
 Definition listUpdate_error{E: Type}(l: list E)(i: nat)(e: E): option (list E) :=
-  if dec (i < length l) then Some (listUpdate l i e) else None.
+  if Nat.ltb i (length l) then Some (listUpdate l i e) else None.
 
 Lemma listUpdate_error_length: forall E i l l' (e: E),
   listUpdate_error l i e = Some l' ->
@@ -107,7 +110,7 @@ Proof.
       eapply IHi with (l := l).
       2: eassumption.
       unfold listUpdate_error.
-      destruct (dec (i < length l)); [reflexivity|bomega].
+      destr (Nat.ltb i (length l)); [reflexivity|bomega].
 Qed.
 
 Lemma nth_error_firstn: forall E i (l: list E) j,
